might work

src/tidy/rewrite_all_2.lean
@@ -1,6 +1,92 @@
+import .lock_tactic_state
+
 open tactic
 
-def f (x : ℕ) := 2
+def f (x : ℕ) (y : ℕ) := 2
+
+meta def repeat_kabstract_core (e : tactic (expr × list expr)) : expr → list (expr × list expr) → tactic (expr × list (expr × list expr))
+| t results := do
+  (e', mvars) ← e,
+  r ← try_core (do r ← kabstract t e', guard r.has_var, return r),
+  match r with
+  | none := return (t, results)
+  | (some t') := do 
+    ty ← infer_type e',
+    -- n ← mk_fresh_name,
+    -- let w := expr.local_const n n binder_info.default ty,
+    w ← mk_meta_var ty,
+    t'' ← return $ t'.instantiate_var w,
+    mvars' ← mvars.mmap instantiate_mvars,
+    repeat_kabstract_core t'' ((w, mvars') :: results)
+  end   
+
+meta def substitutions_core : expr → list expr → 
+  tactic (tactic (expr × list expr) × (list expr → tactic expr) × (list expr → tactic expr))
+| (expr.pi n bi d b) types := 
+  do substitutions_core b (d :: types)          
+| `(%%lhs = %%rhs) types := 
+  do let fresh_mvars := (do mvars ← types.mmap mk_meta_var,
+                           let pattern := lhs.instantiate_vars mvars,
+                           return (pattern, mvars)),
+     let lhs_replacer : list expr → tactic expr := (λ values, return (lhs.instantiate_vars values)),
+     let rhs_replacer : list expr → tactic expr := (λ values, return (rhs.instantiate_vars values)),
+     return (fresh_mvars, lhs_replacer, rhs_replacer)
+| _ _ := failed
+
+/-- Given a lemma `eq`, returns three tactics.
+    1) returning `(lhs', mvars)` where `lhs'` is a copy of the left hand side of the lemma, with
+    variables replaced by fresh metavariables `mvars`.
+    2) taking a list of expressions, and returning `lhs'`, the left hand side with variables
+    instantiated with these values.
+    3) as with 2), but for the right hand side. -/
+meta def substitutions (eq : expr) : tactic (tactic (expr × list expr) × (list expr → tactic expr) × (list expr → tactic expr)) :=
+substitutions_core eq []
+
+universe u
+
+def list.rotate_left {α : Type u} (L : list α) (n : ℕ) := L.drop n ++ L.take n
+
+def list.rotations {α : Type u} (L : list α) : list (list α) :=
+(list.range L.length).map $ λ n, L.rotate_left n
+
+/-- `repeat_kabstract t eq` repeatedly calls `kabstract` on `t`, 
+    looking for subexpressions matching the lhs, after binders, of `eq`. 
+    After each call, the local variable is replaced with a local constant, and the
+    bindings of metavariables in `e` are recorded.
+    
+    The result consists of `(t', L)`, where `t'` is `t` with subexpressions replaced by local
+    constants. The list `L` contains pairs `(n, M)`, where `n` is one of the local constants,
+    and `M` is the list of values of metavariables for that replacement. -/
+meta def repeat_kabstract (t eq : expr) : tactic unit :=
+do (lhs_matcher, lhs_substituter, rhs_substituter) ← substitutions eq,
+  (t', mvars) ← repeat_kabstract_core lhs_matcher t [],
+  trace t',
+  trace mvars,
+  let substituter : list (expr × list expr) → tactic expr := λ mvars,
+    lock_tactic_state $ 
+    (do m_h :: m_t ← return mvars,
+       rhs ← rhs_substituter m_h.2,
+       unify rhs m_h.1,
+       m_t.mmap (λ p, do lhs ← lhs_substituter p.2, unify lhs p.1),
+       instantiate_mvars t'),
+  t' ← mvars.rotations.mmap substituter,
+  -- t' ← substituter mvars,
+  trace t',
+  skip
+
+lemma fx (n : ℕ) (m : ℕ) : f n m = f 17 19 := sorry
+
+example : [f 1 2, 3, f 2 5] = [f 3 1, f 4 1] :=
+begin
+(do `(%%lhs = %%rhs) ← target,
+    trace lhs,
+    eq ← mk_const `fx,
+    trace eq,
+    ty ← infer_type eq,
+    r ← repeat_kabstract lhs ty,
+    trace r
+)
+end
 
 example : f 1 = f 2 :=
 begin
@@ -18,7 +104,14 @@ begin
    a' ← to_expr ``(f _),
    k' ← kabstract k a' transparency.reducible ff,
    trace k',
-   skip),
+   n ← mk_fresh_name,
+   let w := expr.local_const n `w binder_info.default ty,
+   k' ← return $ k'.instantiate_var w,
+   trace k',
+   a'' ← to_expr ``(f _),
+   k'' ← kabstract k' a'' transparency.reducible ff,
+   trace k'',
+skip),
    refl
 end
 
